new subsctipt, unsolvable polymorphic statement

src/alc.lean
@@ -18,11 +18,13 @@ complete. In this file, ACL syntax and semantics are defined.
 namespace ALC
 
 inductive Role (AtomicRole : Type) : Type
-  | Atomic : AtomicRole → Role
+  | Atomic  : AtomicRole → Role
+  | Compose : Role → Role → Role
+  | Inverse : Role → Role
 
 inductive Concept (AtomicConcept AtomicRole : Type) : Type 
-  | TopConcept    : Concept
-  | BottomConcept : Concept
+  | Top           : Concept
+  | Bot           : Concept
   | Atomic        : AtomicConcept → Concept
   | Negation      : Concept → Concept
   | Intersection  : Concept → Concept → Concept
@@ -32,16 +34,30 @@ inductive Concept (AtomicConcept AtomicRole : Type) : Type
 
 open Concept Role
 
-notation        `⊤` := Concept.TopConcept    -- \top
-notation        `⊥` := Concept.BottomConcept -- \bot
-local prefix     `¬` : 51 := Concept.Negation       -- \neg
-local infix      `⊓` : 55 := Concept.Intersection   -- ◾\sqcap
-local infix      `⊔` : 55 := Concept.Union         -- \sqcup
-notation `∃ₐ` R `.ₐ` C := Concept.Some R C -- (it would be nice to use `∃ R. C`)
-notation `∀ₐ` R `.ₐ` C := Concept.Every R C -- (it would be nice to use `∀ R. C`)
+attribute [pattern] has_inf.inf has_sup.sup has_top.top has_bot.bot
+
+instance concept_has_top (AtomicConcept AtomicRole : Type) : 
+ has_top (Concept AtomicConcept AtomicRole) := ⟨ Concept.Top ⟩ 
+
+instance concept_has_bot (AtomicConcept AtomicRole : Type) : 
+ has_bot (Concept AtomicConcept AtomicRole) := ⟨ Concept.Bot ⟩ 
+
+instance concept_has_inf (AtomicConcept AtomicRole : Type) : 
+ has_inf (Concept AtomicConcept AtomicRole) := ⟨ Concept.Intersection ⟩
+
+instance concept_has_sup (AtomicConcept AtomicRole : Type) : 
+ has_sup (Concept AtomicConcept AtomicRole) := ⟨ Concept.Union ⟩
 
 
--- interpretation structure 
+-- local infix     `⊓` : 55 := Concept.Intersection  -- \sqcap
+-- local infix     `⊔` : 55 := Concept.Union         -- \sqcup
+-- notation        `⊤` := Concept.TopConcept    -- \top
+-- notation        `⊥` := Concept.BottomConcept -- \bot
+prefix          `¬ₐ` : 55 := Concept.Negation
+notation `Ex` R `:` C := Concept.Some R C  -- (it would be nice to use `∃ R. C`)
+notation `Ax` R `:` C := Concept.Every R C -- (it would be nice to use `∀ R. C`)
+
+
 structure Interpretation (AtomicConcept AtomicRole : Type) := 
 mk :: (δ : Type) 
       [nonempty : nonempty δ]
@@ -50,28 +66,32 @@ mk :: (δ : Type)
 
 variables {AtomicConcept AtomicRole : Type}
 
+
 -- role interpretation
-definition r_interp (I : Interpretation AtomicConcept AtomicRole) : Role AtomicRole → set (I.δ × I.δ)  
-  | (Role.Atomic R) := I.atom_R R
+def r_interp (I : Interpretation AtomicConcept AtomicRole) : Role AtomicRole → set (I.δ × I.δ)  
+  | (Role.Atomic R)    := I.atom_R R
+  | (Role.Inverse R)   := { d | ∀ x: I.δ × I.δ, x ∈ (r_interp R) → d.1 = x.2 ∧ d.2 = x.1 }
+  | (Role.Compose R S) := { d | ∀ x y : I.δ × I.δ, x ∈ (r_interp R) ∧ y ∈ (r_interp R) ∧ 
+                                  x.2 = y.1 → d.1 =  x.1 ∧ d.2 = y.2 }
 
 -- concept interpretation
-definition interp (I : Interpretation AtomicConcept AtomicRole) : Concept AtomicConcept AtomicRole → set I.δ 
+def interp (I : Interpretation AtomicConcept AtomicRole) : Concept AtomicConcept AtomicRole → set I.δ 
  | ⊤            := univ
  | ⊥            := ∅ 
  | (Atomic C)   := I.atom_C C
- | (¬ C)        := compl (interp C)
- | (C1 ⊓ C2)    := (interp C1) ∩ (interp C2)
+ | (¬ₐ C)       := compl (interp C)
+ | (C1 ⊓ C2)    := (interp C1) ∩ (interp C2) 
  | (C1 ⊔ C2)    := (interp C1) ∪ (interp C2)
- | (Some R C)   := { a: I.δ | ∃ b : I.δ, 
+ | Ex R : C     := { a: I.δ | ∃ b : I.δ, 
                      (a, b) ∈ (r_interp I R) ∧ b ∈ (interp C) }
- | (Every R C)  := { a: I.δ | ∀ b : I.δ,
+ | Ax R : C     := { a: I.δ | ∀ b : I.δ,
                      (a, b) ∈ (r_interp I R) → b ∈ (interp C) }
-
+ 
 
 -- more general properties of 'interp' should also be provable:
 
 lemma interp_inter_neg_empty (a b : Type) (i : Interpretation a b) (c : Concept a b) : 
- interp i (c ⊓ (¬ c)) = ∅ := 
+ interp i (c ⊓ (¬ₐ c)) = ∅ := 
 begin
   dsimp [interp],
   --rw inter_comm,
@@ -79,14 +99,12 @@ begin
   --exact set.compl_inter_self (interp i c),
 end
 
-
 lemma interp_union_neq_univ (a b : Type) (i : Interpretation a b) (c : Concept a b) : 
- interp i (c ⊔ ¬ c) = univ := 
+ interp i (c ⊔ (¬ₐ c)) = univ := 
 begin
   dsimp [interp],
   exact set.union_compl_self (interp i c),
 end
-
 
 def satisfiable (C : Concept AtomicConcept AtomicRole) : Prop :=
   ∃ I : Interpretation AtomicConcept AtomicRole, interp I C ≠ ∅
@@ -97,12 +115,49 @@ def subsumption (C D: Concept AtomicConcept AtomicRole) : Prop :=
 def equivalence (C D: Concept AtomicConcept AtomicRole) : Prop := 
   subsumption C D ∧ subsumption D C
 
-local infix `⊑` : 50 := subsumption -- \sqsubseteq
-local infix `≡` : 50 := equivalence -- \==
+
+local infix ` ⊑  ` : 50 := subsumption
+local infix ` ≡  ` : 50 := equivalence
+
+inductive Statement {AC AR : Type} : Type
+  | Subsumption : Concept AC AR → Concept AC AR → Statement
+  | Equivalence : Concept AC AR → Concept AC AR → Statement
+
+-- Created another operator with a different syntax as the polymorphic instance would not be able
+-- to differentiate beetween the two. Both take Concept AC AR in two instances.
+
+local infix ` ⊑ₛ   ` : 50 := Statement.Subsumption -- \sqsubseteq
+local infix ` ≡ₛ   ` : 50 := Statement.Equivalence -- \==
+
+
+definition interp_stmt {AC AR : Type} (I : Interpretation AC AR) : @Statement AC AR → Prop
+  | (Statement.Subsumption C D) := interp I C ⊆ interp I D
+  | (Statement.Equivalence C D) := interp I C = interp I D
+
+
+def sat_concept_tbox {AC AR : Type} (tbox : set (@Statement AC AR)) (a : @Statement AC AR) : Prop :=
+  ∃ I : Interpretation AC AR,
+    (∀ c ∈ tbox, (interp_stmt I c)) → (interp_stmt I a)
+
+example (ac ar : Type) (A B C : Concept ac ar) : sat_concept_tbox { A ⊑ₛ B , B ⊑ₛ C } (A ⊑ₛ C) := 
+begin
+ unfold sat_concept_tbox,
+ let i : Interpretation ac ar := { Interpretation . 
+    δ := ℕ, 
+    nonempty :=  ⟨0⟩, 
+    atom_C := (λ x : ac, ∅), 
+    atom_R := (λ x : ar, ∅) },
+ existsi i,
+ intro h1,
+ have ha := h1 (A ⊑ₛ B),simp at ha,
+ have hb := h1 (B ⊑ₛ C), simp at hb,
+ unfold interp_stmt at *,
+ exact (subset.trans ha hb),
+end
 
 -- see https://leanprover.zulipchat.com/#narrow/stream/113488-general/topic/non.20empty.20set.20in.20a.20structure
 
-lemma sat_union_neq (a b : Type) (C : Concept a b) : satisfiable (¬ C ⊔ C) :=
+lemma sat_union_neq (a b : Type) (C : Concept a b) : satisfiable ((¬ₐ C) ⊔ C) :=
 begin
   dsimp [satisfiable, interp],
   let i : Interpretation a b := { Interpretation . 
@@ -129,7 +184,7 @@ begin
 end
 
 
-lemma not_sat_inter_neg (a b : Type) (C : Concept a b) : ¬ satisfiable (¬ C ⊓ C) := 
+lemma not_sat_inter_neg (a b : Type) (C : Concept a b) : ¬ satisfiable ((¬ₐ C) ⊓ C) := 
 begin
   dsimp [satisfiable,interp],
   -- don't even need to instatiate
@@ -177,6 +232,12 @@ begin
   exact subset_union_right (interp h C) (interp h D),
 end
 
+lemma subsum_refl (C : Concept AtomicConcept AtomicRole) : C ⊑ C :=
+begin
+  dsimp [subsumption, interp],
+  intro h,
+  exact subset.refl (interp h C), 
+end
 
 lemma subsum_trans (C D E: Concept AtomicConcept AtomicRole) (cd : C ⊑ D) (de : D ⊑ E) : 
    C ⊑ E :=
@@ -188,12 +249,13 @@ begin
   exact (subset.trans h1 h2),
 end 
 
-lemma subsum_refl (C : Concept AtomicConcept AtomicRole) : C ⊑ C :=
+lemma subsum_antisymm (C D : Concept AtomicConcept AtomicRole) (cd : C ⊑  D) (dc : D ⊑  C) : C ≡ D :=
 begin
-  dsimp [subsumption, interp],
-  intro h,
-  exact subset.refl (interp h C), 
-end
+  dsimp[subsumption,equivalence,interp] at *,
+  split,
+  intro h, exact cd h,
+  intro h, exact dc h,
+end 
 
 lemma equiv_refl (C : Concept AtomicConcept AtomicRole) : C ≡ C :=
 begin
@@ -201,9 +263,16 @@ begin
   split,
   exact subsum_refl C, exact subsum_refl C,
 end
-/- 
-1. all concepts C is equivalent to itself
-2. all concepts C \sqsubseteq (subsubmise) ifself
--/
+
+lemma subsum_stat_refl {AC AR : Type} (I : Interpretation AC AR) (C : Concept AC AR) : interp_stmt I (C ⊑ₛ C) :=
+begin
+  unfold interp_stmt,
+end
+
+lemma subsum_stat_trans {AC AR : Type} (I : Interpretation AC AR) (C D E: Concept AC AR) (cd : (C ⊑ₛ D)) (de : D ⊑ₛ E) : 
+   C ⊑ₛ E :=
+begin
+  
+end 
 
 end ALC
